lang/domain.v
@@ -18,6 +18,39 @@ From stdpp Require Import bitvector.definitions.
 (*   Lemma bool_cases (b : Zmod 2) : BoolCases b. *)
 (*   Proof. destruct (Zmod.in_elements b ltac:(inversion 1)); intuition subst; constructor. Qed. *)
 (* End Zmod. *)
+Module Import BV.
+  Coercion embed_bool (b : bool) : bv 1 := bool_to_bv _ b.
+  Coercion nonzero {m} (x : bv m) : bool := negb (bv_unsigned x =? 0)%Z.
+  Lemma nonzero_bool (b : bool) : nonzero b = b :> bool. Proof. case b; trivial. Qed.
+  Inductive Cases2 : bv 1 -> Prop :=
+  | Cases2_0 : Cases2 (Z_to_bv _ 0) | Cases2_1 : Cases2 (Z_to_bv _ 1).
+  Lemma cases2 (x : bv 1) : Cases2 x.
+  Proof.
+    destruct (decide (x = Z_to_bv _ 0)) as [->|Hne].
+    - constructor.
+    - enough (x = Z_to_bv 1 1) as -> by constructor.
+      apply (proj2 (bv_eq _ _ _)).
+      assert (Hne' : bv_unsigned x ≠ 0%Z).
+      { intro He. apply Hne. apply (proj2 (bv_eq _ _ _)).
+        rewrite Z_to_bv_unsigned. exact He.
+        }
+      assert (Heq : bv_unsigned (Z_to_bv 1 1) = 1%Z) by
+        (apply Z_to_bv_small; unfold bv_modulus; simpl; lia).
+      rewrite Heq.
+      pose proof (bv_unsigned_in_range 1 x) as Hr.
+      unfold bv_modulus in Hr. simpl in Hr. lia.
+  Qed.
+  Inductive BoolCases : bv 1 -> Prop :=
+  | BoolTrue : BoolCases true | BoolFalse : BoolCases false.
+  Lemma bool_cases (b : bv 1) : BoolCases b.
+  Proof.
+    destruct (cases2 b).
+    - enough (embed_bool false = Z_to_bv _ 0) as H by (rewrite <- H; exact BoolFalse).
+      apply (proj2 (bv_eq _ _ _)).
+      vm_compute. reflexivity.
+    - exact BoolTrue.
+  Qed.
+End BV.
 
 Module bits.
   Definition hex {n : N} (v : bv n) : string :=
